removing the type info from the rec constructor

process/processes.v
@@ -12,7 +12,7 @@ Inductive process  : Type :=
   | p_send : ( part   ) -> ( label   ) -> ( expr   ) -> ( process   ) -> process 
   | p_recv : ( part   ) -> ( list (prod (prod (label  ) (sort  )) (process  )) ) -> process 
   | p_ite : ( expr   ) -> ( process   ) -> ( process   ) -> process 
-  | p_rec : ( ltt   ) -> ( process   ) -> process .
+  | p_rec : ( process   ) -> process .
 
 Lemma congr_p_inact  : p_inact  = p_inact  .
 Proof. congruence. Qed.
@@ -26,7 +26,7 @@ Proof. congruence. Qed.
 Lemma congr_p_ite  { s0 : expr   } { s1 : process   } { s2 : process   } { t0 : expr   } { t1 : process   } { t2 : process   } (H1 : s0 = t0) (H2 : s1 = t1) (H3 : s2 = t2) : p_ite  s0 s1 s2 = p_ite  t0 t1 t2 .
 Proof. congruence. Qed.
 
-Lemma congr_p_rec  { s0 : ltt   } { s1 : process   } { t0 : ltt   } { t1 : process   } (H1 : s0 = t0) (H2 : s1 = t1) : p_rec  s0 s1 = p_rec  t0 t1 .
+Lemma congr_p_rec  { s1 : process   } { t1 : process   }  (H2 : s1 = t1) : p_rec  s1 = p_rec t1 .
 Proof. congruence. Qed.
 
 Definition upRen_process_process   (xi : ( fin ) -> fin) : ( fin ) -> fin :=
@@ -39,7 +39,7 @@ Fixpoint ren_process   (xiprocess : ( fin ) -> fin) (s : process ) : process  :=
     | p_send  s0 s1 s2 s3 => p_send  ((fun x => x) s0) ((fun x => x) s1) ((fun x => x) s2) ((ren_process xiprocess) s3)
     | p_recv  s0 s1 => p_recv  ((fun x => x) s0) ((list_map (prod_map (prod_map (fun x => x) (fun x => x)) (ren_process xiprocess))) s1)
     | p_ite  s0 s1 s2 => p_ite  ((fun x => x) s0) ((ren_process xiprocess) s1) ((ren_process xiprocess) s2)
-    | p_rec  s0 s1 => p_rec  ((fun x => x) s0) ((ren_process (upRen_process_process xiprocess)) s1)
+    | p_rec  s1 => p_rec ((ren_process (upRen_process_process xiprocess)) s1)
     end.
 
 Definition up_process_process   (sigma : ( fin ) -> process ) : ( fin ) -> process  :=
@@ -52,9 +52,8 @@ Fixpoint subst_process   (sigmaprocess : ( fin ) -> process ) (s : process ) : p
     | p_send  s0 s1 s2 s3 => p_send  ((fun x => x) s0) ((fun x => x) s1) ((fun x => x) s2) ((subst_process sigmaprocess) s3)
     | p_recv  s0 s1 => p_recv  ((fun x => x) s0) ((list_map (prod_map (prod_map (fun x => x) (fun x => x)) (subst_process sigmaprocess))) s1)
     | p_ite  s0 s1 s2 => p_ite  ((fun x => x) s0) ((subst_process sigmaprocess) s1) ((subst_process sigmaprocess) s2)
-    | p_rec  s0 s1 => p_rec  ((fun x => x) s0) ((subst_process (up_process_process sigmaprocess)) s1)
+    | p_rec s1 => p_rec ((subst_process (up_process_process sigmaprocess)) s1)
     end.
-
 
 Definition isNil {A: Type} (l: list A): bool :=
   match l with
@@ -73,9 +72,41 @@ Fixpoint unfold_rec (s: process): process :=
         end
       in p_recv a (next l)
     | p_ite e p1 p2  => p_ite e (unfold_rec p1) (unfold_rec p2)
-    | p_rec l0 p     => subst_process ((p_rec l0 p) .: p_var) p
+    | p_rec p     => subst_process ((p_rec p) .: p_var) p
     | _              => s
   end.
+
+Fixpoint subst_proc (q p: process): process :=
+  match p with
+    | p_var s        => p_var s 
+    | p_recv pt xs   => p_recv pt ((list_map (prod_map (prod_map (fun x => x) (fun x => x)) (subst_proc q))) xs)
+    | p_ite e1 P Q   => p_ite e1 (subst_proc q P) (subst_proc q Q)
+    | p_send a l e P => p_send a l e (subst_proc q P)
+    | p_rec P        => p_rec (subst_process (q .: p_var) P) 
+    | p_inact        => p_inact
+  end.
+
+Let pr1: process := p_rec (p_rec (p_rec (p_var 88))).
+Eval compute in subst_proc (p_var 10) pr1.
+
+Fixpoint subst_proc_var (n: fin) (p: process): process :=
+  match p with
+    | p_var s        => p_var s 
+    | p_recv pt xs   => p_recv pt ((list_map (prod_map (prod_map (fun x => x) (fun x => x)) (subst_proc_var n))) xs)
+    | p_ite e1 P Q   => p_ite e1 (subst_proc_var n P) (subst_proc_var n Q)
+    | p_send a l e P => p_send a l e (subst_proc_var n P)
+    | p_rec P        => p_rec (subst_process ((p_var n) .: p_var) P) 
+    | p_inact        => p_inact
+  end.
+
+(*
+Let pr1: process := p_rec (ltt_end) (p_var 0).
+Eval compute in subst_proc_var 2 pr1.
+*)
+
+(*
+Let pr1: process := p_rec (ltt_end) (p_rec (ltt_end) (p_rec (ltt_end) (p_var 2))).
+Eval compute in subst_proc p_inact pr1. *)
 
 (* Inductive p_cong: relation process :=
   | p_cong_rec: forall p, p_cong (p_rec p) (unfold_rec (p_rec p)). *)
@@ -84,7 +115,7 @@ Fixpoint subst_expr_proc_all (e: expr) (p: process): process :=
   match p with
     | p_send pt l e1 P => p_send pt l (subst_expr (e .: e_var) e1) (subst_expr_proc_all e P)
     | p_ite e1 P Q     => p_ite (subst_expr (e .: e_var) e1) (subst_expr_proc_all e P) (subst_expr_proc_all e Q)
-    | p_rec T P        => p_rec T (subst_expr_proc_all e P)
+    | p_rec  P         => p_rec (subst_expr_proc_all e P)
     | p_recv pt xs     => p_recv pt ((list_map (prod_map (prod_map (fun x => x) (fun x => x)) (subst_expr_proc_all e))) xs)
     | _                => p
   end.
@@ -101,7 +132,7 @@ Definition subst_expr_proc (p: process) (l: label) (e: expr): process :=
               | p_send pt l e1 P => p_send pt l (subst_expr (e .: e_var) e1) (rec P)
               | p_ite e1 P Q     => p_ite (subst_expr (e .: e_var) e1) (rec P) (rec Q)
               | p_recv s2 s3     => p_recv s2 ((list_map (prod_map (prod_map (fun x => x) (fun x => x)) (rec))) s3)
-              | p_rec l0 P       => p_rec l0 (rec P)
+              | p_rec P          => p_rec (rec P)
               | _                => P
             end
           in rec P
@@ -113,11 +144,11 @@ Definition subst_expr_proc (p: process) (l: label) (e: expr): process :=
   end.
 
 (*
-Definition pp := p_recv "A" [("l1", sint,
-                                (p_recv "B" [("l2", sint, 
-                                             (p_send "A" "l3" (e_gt (e_var 0) (e_var 0)) p_inact))]))].
+Definition pp := p_recv "A" [(1, sint,
+                                (p_recv "B" [(2, sint, 
+                                             (p_send "A" 3 (e_gt (e_var 1) (e_var 0)) p_inact))]))].
 
-Eval compute in (subst_expr_proc pp "l1" (e_val (vint (10%Z)))). *)
+Eval compute in (subst_expr_proc pp 1 (e_val (vint (10%Z)))). *)
 
 (* Let pp := p_rec (p_send "p" "l" (e_var "x") (p_var 0)).
 Let pp2 := Eval simpl in unfold_rec pp.
@@ -140,7 +171,7 @@ Fixpoint idSubst_process  (sigmaprocess : ( fin ) -> process ) (Eqprocess : fora
     | p_send  s0 s1 s2 s3 => congr_p_send ((fun x => (eq_refl) x) s0) ((fun x => (eq_refl) x) s1) ((fun x => (eq_refl) x) s2) ((idSubst_process sigmaprocess Eqprocess) s3)
     | p_recv  s0 s1 => congr_p_recv ((fun x => (eq_refl) x) s0) ((list_id (prod_id (prod_id (fun x => (eq_refl) x) (fun x => (eq_refl) x)) (idSubst_process sigmaprocess Eqprocess))) s1)
     | p_ite  s0 s1 s2 => congr_p_ite ((fun x => (eq_refl) x) s0) ((idSubst_process sigmaprocess Eqprocess) s1) ((idSubst_process sigmaprocess Eqprocess) s2)
-    | p_rec  s0 s1 => congr_p_rec ((fun x => (eq_refl) x) s0) ((idSubst_process (up_process_process sigmaprocess) (upId_process_process (_) Eqprocess)) s1)
+    | p_rec s1 => congr_p_rec ((idSubst_process (up_process_process sigmaprocess) (upId_process_process (_) Eqprocess)) s1)
     end.
 
 Definition upExtRen_process_process   (xi : ( fin ) -> fin) (zeta : ( fin ) -> fin) (Eq : forall x, xi x = zeta x) : forall x, (upRen_process_process xi) x = (upRen_process_process zeta) x :=
@@ -156,7 +187,7 @@ Fixpoint extRen_process   (xiprocess : ( fin ) -> fin) (zetaprocess : ( fin ) ->
     | p_send  s0 s1 s2 s3 => congr_p_send ((fun x => (eq_refl) x) s0) ((fun x => (eq_refl) x) s1) ((fun x => (eq_refl) x) s2) ((extRen_process xiprocess zetaprocess Eqprocess) s3)
     | p_recv  s0 s1 => congr_p_recv ((fun x => (eq_refl) x) s0) ((list_ext (prod_ext (prod_ext (fun x => (eq_refl) x) (fun x => (eq_refl) x)) (extRen_process xiprocess zetaprocess Eqprocess))) s1)
     | p_ite  s0 s1 s2 => congr_p_ite ((fun x => (eq_refl) x) s0) ((extRen_process xiprocess zetaprocess Eqprocess) s1) ((extRen_process xiprocess zetaprocess Eqprocess) s2)
-    | p_rec  s0 s1 => congr_p_rec ((fun x => (eq_refl) x) s0) ((extRen_process (upRen_process_process xiprocess) (upRen_process_process zetaprocess) (upExtRen_process_process (_) (_) Eqprocess)) s1)
+    | p_rec  s1 => congr_p_rec  ((extRen_process (upRen_process_process xiprocess) (upRen_process_process zetaprocess) (upExtRen_process_process (_) (_) Eqprocess)) s1)
     end.
 
 Definition upExt_process_process   (sigma : ( fin ) -> process ) (tau : ( fin ) -> process ) (Eq : forall x, sigma x = tau x) : forall x, (up_process_process sigma) x = (up_process_process tau) x :=
@@ -172,7 +203,7 @@ Fixpoint ext_process   (sigmaprocess : ( fin ) -> process ) (tauprocess : ( fin 
     | p_send  s0 s1 s2 s3 => congr_p_send ((fun x => (eq_refl) x) s0) ((fun x => (eq_refl) x) s1) ((fun x => (eq_refl) x) s2) ((ext_process sigmaprocess tauprocess Eqprocess) s3)
     | p_recv  s0 s1 => congr_p_recv ((fun x => (eq_refl) x) s0) ((list_ext (prod_ext (prod_ext (fun x => (eq_refl) x) (fun x => (eq_refl) x)) (ext_process sigmaprocess tauprocess Eqprocess))) s1)
     | p_ite  s0 s1 s2 => congr_p_ite ((fun x => (eq_refl) x) s0) ((ext_process sigmaprocess tauprocess Eqprocess) s1) ((ext_process sigmaprocess tauprocess Eqprocess) s2)
-    | p_rec  s0 s1 => congr_p_rec ((fun x => (eq_refl) x) s0) ((ext_process (up_process_process sigmaprocess) (up_process_process tauprocess) (upExt_process_process (_) (_) Eqprocess)) s1)
+    | p_rec s1 => congr_p_rec ((ext_process (up_process_process sigmaprocess) (up_process_process tauprocess) (upExt_process_process (_) (_) Eqprocess)) s1)
     end.
 
 Definition up_ren_ren_process_process    (xi : ( fin ) -> fin) (tau : ( fin ) -> fin) (theta : ( fin ) -> fin) (Eq : forall x, ((funcomp) tau xi) x = theta x) : forall x, ((funcomp) (upRen_process_process tau) (upRen_process_process xi)) x = (upRen_process_process theta) x :=
@@ -185,7 +216,7 @@ Fixpoint compRenRen_process    (xiprocess : ( fin ) -> fin) (zetaprocess : ( fin
     | p_send  s0 s1 s2 s3 => congr_p_send ((fun x => (eq_refl) x) s0) ((fun x => (eq_refl) x) s1) ((fun x => (eq_refl) x) s2) ((compRenRen_process xiprocess zetaprocess rhoprocess Eqprocess) s3)
     | p_recv  s0 s1 => congr_p_recv ((fun x => (eq_refl) x) s0) ((list_comp (prod_comp (prod_comp (fun x => (eq_refl) x) (fun x => (eq_refl) x)) (compRenRen_process xiprocess zetaprocess rhoprocess Eqprocess))) s1)
     | p_ite  s0 s1 s2 => congr_p_ite ((fun x => (eq_refl) x) s0) ((compRenRen_process xiprocess zetaprocess rhoprocess Eqprocess) s1) ((compRenRen_process xiprocess zetaprocess rhoprocess Eqprocess) s2)
-    | p_rec  s0 s1 => congr_p_rec ((fun x => (eq_refl) x) s0) ((compRenRen_process (upRen_process_process xiprocess) (upRen_process_process zetaprocess) (upRen_process_process rhoprocess) (up_ren_ren (_) (_) (_) Eqprocess)) s1)
+    | p_rec  s1 => congr_p_rec ((compRenRen_process (upRen_process_process xiprocess) (upRen_process_process zetaprocess) (upRen_process_process rhoprocess) (up_ren_ren (_) (_) (_) Eqprocess)) s1)
     end.
 
 Definition up_ren_subst_process_process    (xi : ( fin ) -> fin) (tau : ( fin ) -> process ) (theta : ( fin ) -> process ) (Eq : forall x, ((funcomp) tau xi) x = theta x) : forall x, ((funcomp) (up_process_process tau) (upRen_process_process xi)) x = (up_process_process theta) x :=
@@ -201,8 +232,7 @@ Fixpoint compRenSubst_process    (xiprocess : ( fin ) -> fin) (tauprocess : ( fi
     | p_send  s0 s1 s2 s3 => congr_p_send ((fun x => (eq_refl) x) s0) ((fun x => (eq_refl) x) s1) ((fun x => (eq_refl) x) s2) ((compRenSubst_process xiprocess tauprocess thetaprocess Eqprocess) s3)
     | p_recv  s0 s1 => congr_p_recv ((fun x => (eq_refl) x) s0) ((list_comp (prod_comp (prod_comp (fun x => (eq_refl) x) (fun x => (eq_refl) x)) (compRenSubst_process xiprocess tauprocess thetaprocess Eqprocess))) s1)
     | p_ite  s0 s1 s2 => congr_p_ite ((fun x => (eq_refl) x) s0) ((compRenSubst_process xiprocess tauprocess thetaprocess Eqprocess) s1) ((compRenSubst_process xiprocess tauprocess thetaprocess Eqprocess) s2)
-    | p_rec  s0 s1 => congr_p_rec ((fun x => (eq_refl) x) s0) ((compRenSubst_process (upRen_process_process xiprocess) (up_process_process tauprocess) (up_process_process thetaprocess) (up_ren_subst_process_process (_) (_) (_) Eqprocess)) s1)
-    end.
+    | p_rec  s1 => congr_p_rec  ((compRenSubst_process (upRen_process_process xiprocess) (up_process_process tauprocess) (up_process_process thetaprocess) (up_ren_subst_process_process (_) (_) (_) Eqprocess)) s1)   end.
 
 Definition up_subst_ren_process_process    (sigma : ( fin ) -> process ) (zetaprocess : ( fin ) -> fin) (theta : ( fin ) -> process ) (Eq : forall x, ((funcomp) (ren_process zetaprocess) sigma) x = theta x) : forall x, ((funcomp) (ren_process (upRen_process_process zetaprocess)) (up_process_process sigma)) x = (up_process_process theta) x :=
   fun n => match n with
@@ -217,7 +247,7 @@ Fixpoint compSubstRen_process    (sigmaprocess : ( fin ) -> process ) (zetaproce
     | p_send  s0 s1 s2 s3 => congr_p_send ((fun x => (eq_refl) x) s0) ((fun x => (eq_refl) x) s1) ((fun x => (eq_refl) x) s2) ((compSubstRen_process sigmaprocess zetaprocess thetaprocess Eqprocess) s3)
     | p_recv  s0 s1 => congr_p_recv ((fun x => (eq_refl) x) s0) ((list_comp (prod_comp (prod_comp (fun x => (eq_refl) x) (fun x => (eq_refl) x)) (compSubstRen_process sigmaprocess zetaprocess thetaprocess Eqprocess))) s1)
     | p_ite  s0 s1 s2 => congr_p_ite ((fun x => (eq_refl) x) s0) ((compSubstRen_process sigmaprocess zetaprocess thetaprocess Eqprocess) s1) ((compSubstRen_process sigmaprocess zetaprocess thetaprocess Eqprocess) s2)
-    | p_rec  s0 s1 => congr_p_rec ((fun x => (eq_refl) x) s0) ((compSubstRen_process (up_process_process sigmaprocess) (upRen_process_process zetaprocess) (up_process_process thetaprocess) (up_subst_ren_process_process (_) (_) (_) Eqprocess)) s1)
+    | p_rec  s1 => congr_p_rec  ((compSubstRen_process (up_process_process sigmaprocess) (upRen_process_process zetaprocess) (up_process_process thetaprocess) (up_subst_ren_process_process (_) (_) (_) Eqprocess)) s1)
     end.
 
 Definition up_subst_subst_process_process    (sigma : ( fin ) -> process ) (tauprocess : ( fin ) -> process ) (theta : ( fin ) -> process ) (Eq : forall x, ((funcomp) (subst_process tauprocess) sigma) x = theta x) : forall x, ((funcomp) (subst_process (up_process_process tauprocess)) (up_process_process sigma)) x = (up_process_process theta) x :=
@@ -233,7 +263,7 @@ Fixpoint compSubstSubst_process    (sigmaprocess : ( fin ) -> process ) (tauproc
     | p_send  s0 s1 s2 s3 => congr_p_send ((fun x => (eq_refl) x) s0) ((fun x => (eq_refl) x) s1) ((fun x => (eq_refl) x) s2) ((compSubstSubst_process sigmaprocess tauprocess thetaprocess Eqprocess) s3)
     | p_recv  s0 s1 => congr_p_recv ((fun x => (eq_refl) x) s0) ((list_comp (prod_comp (prod_comp (fun x => (eq_refl) x) (fun x => (eq_refl) x)) (compSubstSubst_process sigmaprocess tauprocess thetaprocess Eqprocess))) s1)
     | p_ite  s0 s1 s2 => congr_p_ite ((fun x => (eq_refl) x) s0) ((compSubstSubst_process sigmaprocess tauprocess thetaprocess Eqprocess) s1) ((compSubstSubst_process sigmaprocess tauprocess thetaprocess Eqprocess) s2)
-    | p_rec  s0 s1 => congr_p_rec ((fun x => (eq_refl) x) s0) ((compSubstSubst_process (up_process_process sigmaprocess) (up_process_process tauprocess) (up_process_process thetaprocess) (up_subst_subst_process_process (_) (_) (_) Eqprocess)) s1)
+    | p_rec  s1 => congr_p_rec ((compSubstSubst_process (up_process_process sigmaprocess) (up_process_process tauprocess) (up_process_process thetaprocess) (up_subst_subst_process_process (_) (_) (_) Eqprocess)) s1)
     end.
 
 Definition rinstInst_up_process_process   (xi : ( fin ) -> fin) (sigma : ( fin ) -> process ) (Eq : forall x, ((funcomp) (p_var ) xi) x = sigma x) : forall x, ((funcomp) (p_var ) (upRen_process_process xi)) x = (up_process_process sigma) x :=
@@ -249,7 +279,7 @@ Fixpoint rinst_inst_process   (xiprocess : ( fin ) -> fin) (sigmaprocess : ( fin
     | p_send  s0 s1 s2 s3 => congr_p_send ((fun x => (eq_refl) x) s0) ((fun x => (eq_refl) x) s1) ((fun x => (eq_refl) x) s2) ((rinst_inst_process xiprocess sigmaprocess Eqprocess) s3)
     | p_recv  s0 s1 => congr_p_recv ((fun x => (eq_refl) x) s0) ((list_ext (prod_ext (prod_ext (fun x => (eq_refl) x) (fun x => (eq_refl) x)) (rinst_inst_process xiprocess sigmaprocess Eqprocess))) s1)
     | p_ite  s0 s1 s2 => congr_p_ite ((fun x => (eq_refl) x) s0) ((rinst_inst_process xiprocess sigmaprocess Eqprocess) s1) ((rinst_inst_process xiprocess sigmaprocess Eqprocess) s2)
-    | p_rec  s0 s1 => congr_p_rec ((fun x => (eq_refl) x) s0) ((rinst_inst_process (upRen_process_process xiprocess) (up_process_process sigmaprocess) (rinstInst_up_process_process (_) (_) Eqprocess)) s1)
+    | p_rec  s1 => congr_p_rec ((rinst_inst_process (upRen_process_process xiprocess) (up_process_process sigmaprocess) (rinstInst_up_process_process (_) (_) Eqprocess)) s1)
     end.
 
 Lemma rinstInst_process   (xiprocess : ( fin ) -> fin) : ren_process xiprocess = subst_process ((funcomp) (p_var ) xiprocess) .
