process/typecheck.v
@@ -12,21 +12,17 @@ Inductive ctx: Type :=
 
 Fixpoint memS (n: fin) (s: sort) (m: ctx): Prop :=
   match m with
-    | consS u v m1 => (n = u /\ v = s) \/ memS n s m1
+    | consS u v m1 => (n = u /\ (exists s', v = s' /\ subsort s s') \/ v = s) \/ memS n s m1
     | consT u v m1 => memS n s m1
     | _            => False
   end.
 
 Fixpoint memT (n: fin) (t: ltt) (m: ctx): Prop :=
   match m with
-    | consT u v m1 => (n = u /\ v = t) \/ memT n t m1
+    | consT u v m1 => (n = u /\ (exists t', v = t' /\ subtypeC t t') \/ v = t) \/ memT n t m1
     | consS u v m1 => memT n t m1
     | _            => False
   end.
-
-Definition eq_ctx (m1 m2: ctx) := 
-  (forall n s, memS n s m1 <-> memS n s m2) /\
-  (forall n t, memT n t m1 <-> memT n t m2).
 
 Definition extendS (m: ctx) (s: fin) (t: expressions.sort) :=
   consS s t m.
@@ -92,6 +88,25 @@ Fixpoint infr_expr (m: ctx) (e: expr): option sort :=
       end
   end.
 
+Inductive subCtx: ctx -> ctx -> Prop :=
+  | sctx1: forall m t t' c c', subCtx c c' -> subtypeC t t' -> subCtx (consT m t c) (consT m t' c')
+  | sctx2: forall m t c c', subCtx c c' -> subCtx (consT m t c) (consT m t c')
+  | sctx3: forall m s s' c c', subCtx c c' -> subsort s s' -> subCtx (consS m s c) (consS m s' c')
+  | sctx4: forall m s c c', subCtx c c' -> subCtx (consS m s c) (consS m s c')
+  | subctxr: forall c, subCtx c c. 
+
+Fixpoint refCtxT (c1 c2: ctx): Prop :=
+  match (c1, c2) with
+    | (consT u1 v1 m1, consT u2 v2 m2) => ((u1 = u2 /\ exists t', v2 = t' /\ subtypeC v1 t') \/ v1 = v2) /\ refCtxT m1 m2
+    | (consS u1 v1 m1, consS u2 v2 m2) => ((u1 = u2 /\ exists s', v2 = s' /\ subsort  v1 s') \/ v1 = v2) /\ refCtxT m1 m2
+    | (empty, empty)                   => True
+    | _                                => False
+  end.
+
+Definition eq_ctx (m1 m2: ctx) := 
+  (forall n s, memS n s m1 <-> memS n s m2) /\
+  (forall n t, memT n t m1 <-> memT n t m2).
+
 Inductive typ_expr: ctx -> expr -> sort -> Prop :=
   | sc_var : forall c s t, Some t = lookupS c s -> typ_expr c (e_var s) t
   | sc_vali: forall c i, typ_expr c (e_val (vint i)) sint
@@ -101,9 +116,10 @@ Inductive typ_expr: ctx -> expr -> sort -> Prop :=
                          typ_expr c (e_succ e) snat
   | sc_neg : forall c e, typ_expr c e sint ->
                          typ_expr c (e_neg e) sint
-  | sc_sub : forall c e s s', typ_expr c e s ->
-                              subsort s s' ->
-                              typ_expr c e s'
+  | sc_sub : forall c c' e s s', typ_expr c e s ->
+                                 subsort s s' ->
+                                 refCtxT c c' ->
+                                 typ_expr c' e s'
   | sc_not : forall c e, typ_expr c e sbool ->
                          typ_expr c (e_not e) sbool
   | sc_gt  : forall c e1 e2, typ_expr c e1 sint ->
@@ -119,20 +135,36 @@ Fixpoint matchSel (l: label) (xs: list(label*(expressions.sort)*ltt)%type): opti
     | (lbl,s,t)::ys => if Nat.eqb l lbl then Some(s,t) else matchSel l ys
   end.
 
+(* Require Import Coq.Init.Logic. *)
+
+(* Definition sub_ctx (m1 m2: ctx) :=
+  ((forall n s s', subsort s s'  -> (memS n s m1 <-> memS n s' m2)) \/ eq_ctx m1 m2) /\
+  ((forall n t t', subtypeC t t' -> (memT n t m1 <-> memT n t' m2)) \/ eq_ctx m1 m2). *)
+
+Definition IF_then_else (P Q R:Prop) := P /\ Q \/ ~ P /\ R.
+
+Fixpoint findCtx (n: fin) (t: ltt) (m: ctx): Prop :=
+  match m with
+    | consT u v m1 => (n = u /\ v = t) \/ findCtx n t m1
+    | consS u v m1 => findCtx n t m1
+    | _            => False
+  end.
+
 Inductive typ_proc: fin -> fin -> ctx -> process -> ltt -> Prop :=
   | tc_inact: forall m em c, typ_proc m em c (p_inact) (ltt_end)
   | tc_var  : forall m em c s t, Some t = lookupT c s ->
                                  typ_proc m em c (p_var s) t
   | tc_mu   : forall m em c p t, let c' := extendT c m t in
                                  typ_proc (S m) em c' p t ->
-                                 typ_proc m em c (p_rec t p) t
+                                 typ_proc m em c (p_rec p) t
   | tc_ite  : forall m em c e p1 p2 T, typ_expr c e sbool ->
                                        typ_proc m em c p1 T ->
                                        typ_proc m em c p2 T ->
                                        typ_proc m em c (p_ite e p1 p2) T
-  | tc_sub  : forall m em c p t t', typ_proc m em c p t ->
-                                    subtypeC t t' ->
-                                    typ_proc m em c p t'
+  | tc_sub  : forall m em c c' p t t', typ_proc m em c p t ->
+                                       subtypeC t t' ->
+                                       refCtxT c c' -> 
+                                       typ_proc m em c' p t'
   | tc_recv : forall m em c p L ST P T,
                      length L = length ST ->
                      length ST = length P ->
@@ -142,6 +174,28 @@ Inductive typ_proc: fin -> fin -> ctx -> process -> ltt -> Prop :=
   | tc_send: forall m em c p l e P S T, typ_expr c e S ->
                                         typ_proc m em c P T ->
                                         typ_proc m em c (p_send p l e P) (ltt_send p [(l,S,T)]).
+
+
+Lemma _a23_d: forall P m em Q T G,
+  typ_proc m em G P T ->
+  (P = (p_rec Q) -> typ_proc (S m) em (extendT G m T) Q T).
+Proof. intros.
+       induction H; intros; try easy.
+       inversion H0.
+       subst.
+(*        destruct H0 as (Ha, Hb). *)
+(*        inversion Ha. subst.  *)
+       unfold c' in *.
+       easy.
+
+       specialize(tc_sub (S m) em (extendT c m t) (extendT c' m t') Q t t'); intro Hs.
+       apply Hs.
+       apply IHtyp_proc. easy. easy.
+       simpl.
+       split. left. split. easy.
+       exists t'. split; easy.
+       easy.
+Qed.
 
 Definition PBob: process := p_recv "Alice" [(1, snat, p_send "Carol" 2 (e_val (vnat 100)) p_inact);
                                             (4, snat, p_send "Carol" 2 (e_val (vnat 2)) p_inact)].
@@ -258,6 +312,34 @@ Proof. intros A B l1.
          apply IHl1. easy.
 Qed.
 
+(* Lemma ref_ctx_1: forall c c' t t' u,
+ refCtxT t t' c c' -> refCtxT u u c c'.
+Proof. intro c.
+       induction c; intros.
+       - case_eq c'; intros.
+         + easy.
+         + subst. simpl in H. easy.
+         + subst. simpl in H. easy.
+       - case_eq c'; intros.
+         + subst. simpl in H. simpl. easy.
+         + subst. simpl. simpl in H.
+           destruct H as (Ha, (Hb, Hc)).
+           subst. split. easy. split. easy.
+           apply IHc with (t := t) (t' := t'). easy.
+         + subst. simpl in H. easy.
+       - case_eq c'; intros.
+         + subst. simpl in H. simpl. easy.
+         + subst. simpl in H. easy.
+         + subst. simpl. simpl in H.
+           destruct H as (Ha, Hb).
+           destruct Ha as [Ha | Ha].
+           destruct Ha as (Ha,(Hc,Hd)).
+           subst.
+           
+           subst. split. easy. split. easy.
+           apply IHc with (t := t) (t' := t'). easy. *)
+
+
 Lemma _a23_a: forall m em p L S Q P G T, 
   typ_proc m em G P T ->
   P = (p_recv p (zip (zip L S) Q)) -> 
@@ -271,7 +353,10 @@ Proof. intros.
        split.
        specialize(IHtyp_proc Hla1 Hla2 Hla3).
        destruct IHtyp_proc as (IHtyp_proc, Ha).
-       specialize(stTrans (ltt_recv p (zip (zip L S) T')) t t' IHtyp_proc H1); intro HT. easy.
+       specialize(stTrans (ltt_recv p (zip (zip L S) T')) t t' IHtyp_proc); intro HT.
+       apply HT.
+       
+        easy.
        
        (**)
        destruct IHtyp_proc as (IHtyp_proc, Ha). easy. easy. easy.
@@ -280,9 +365,14 @@ Proof. intros.
        simpl in *.
        rewrite Forall_forall in Ha.
        specialize(Ha (x1,(x2,x3))). simpl in Ha.
+       specialize(tc_sub m (Datatypes.S em) (extendS c em x1) (extendS c' em x1) x2 x3 x3); intro HTC.
+       apply HTC.
+(*        specialize(tc_sub m (Datatypes.S em) c); intro HTC. *)
        apply Ha. easy.
-       (**)
-       
+       apply stRefl.
+       simpl.
+       split. right. easy. easy.
+
        rewrite Forall_forall in H3.
        exists T.
        intros Hla1 Hla2 Hla3.
@@ -476,10 +566,16 @@ Lemma _a23_b: forall m em p l e Q P G T,
   (P = (p_send p l e Q) -> exists S S' T', typ_expr G e S /\ typ_proc m em G Q T' /\ subsort S' S /\ subtypeC (ltt_send p [(l,S',T')]) T).
 Proof. intros m em p l e Q P G T H.
        induction H; intros; try easy.
-       specialize(IHtyp_proc H1).
+       specialize(IHtyp_proc H2).
        destruct IHtyp_proc as (S,(S',(T',Ha))).
        exists S. exists S'. exists T'.
-       split. easy. split. easy. split. easy.
+       split.
+       specialize(sc_sub c c' e S S); intro HSS.
+       apply HSS. easy. apply srefl. easy.
+       split.
+       specialize(tc_sub m em c c' Q T' T'); intro HTS.
+       apply HTS. easy.
+       apply stRefl. easy. split. easy.
        destruct Ha as (Ha,(Hb,(Hc,Hd))).
        specialize(stTrans (ltt_send p [(l, S', T')]) t t' Hd H0); intro HT.
        apply HT.
@@ -520,31 +616,21 @@ Proof. intros.
        specialize(IHtyp_proc H0).
        destruct IHtyp_proc as (T1,(T2,(Ha,(Hb,(Hc,Hd))))).
        exists T1. exists T2.
-       split. easy. split. easy.
+       split.
+       specialize(tc_sub m em c c' Q1 T1 T1); intro HTS.
+       apply HTS. easy. apply stRefl. easy. 
+       split.
+       specialize(tc_sub m em c c' Q2 T2 T2); intro HTS.
+       apply HTS. easy. apply stRefl. easy. 
        split.
        specialize(stTrans T1 t t' Hc H1); intro HT. easy.
        specialize(stTrans T2 t t' Hd H1); intro HT. easy.
 Qed.
 
-Lemma _a23_d: forall P m em Q T T' G,
-  typ_proc m em G P T ->
-  (P = (p_rec T' Q) /\ subtypeC T T' -> typ_proc (S m) em (extendT G m T') Q T').
-Proof. intros.
-       induction H; intros; try easy.
-       destruct H0 as (Ha, Hb).
-       inversion Ha. subst. 
-       unfold c' in *.
-       easy.
 
-       destruct H0 as (Ha, Hb).
-       specialize(stTrans t t' T' H1 Hb); intro HT.
-       apply IHtyp_proc.
-       split; easy.
-Qed.
-
-Lemma _a23_d_v2: forall P m em Q T G,
+(* Lemma _a23_d_v2: forall P m em Q T G,
   typ_proc m em G P T ->
-  (exists T', (P = (p_rec T' Q) /\ subtypeC T T') -> typ_proc (S m) em (extendT G m T') Q T').
+  (exists T', (P = (p_rec Q) /\ subtypeC T T') -> typ_proc (S m) em (extendT G m T') Q T').
 Proof. intros.
        induction H; try (exists ltt_end; easy).
        exists t.
@@ -561,7 +647,7 @@ Proof. intros.
        specialize(stTrans t t' T' H0 Hb); intro HT.
        exact HT.
 Qed.
-
+ *)
 Lemma _a23_e: forall P (n: fin) m em n T G,
   typ_proc m em G P T ->
   (P = (p_var n) -> exists T' G', eq_ctx G (extendT G' n T') /\ subtypeC T' T).
@@ -576,24 +662,31 @@ Proof. intros.
        exists  T'. exists (consS n1 s G').
 
        split.
-       unfold eq_ctx in *.
+       unfold extendT.
+       unfold eq_ctx in *. 
        split.
        intros. simpl.
        destruct Ha as (Ha1,Ha2).
        split. intro HH.
-       inversion HH.
-       destruct H1 as( H1a, H1b).
+       destruct HH as [HH | HH].
+       destruct HH as [HH | HH].
+       destruct HH as( H1a, H1b).
        subst. unfold extendT. simpl.
-       left. split. easy. easy.
-       simpl. right.
+       left. left. split. easy. easy.
+       left. right. easy.
+       right.
        apply Ha1. easy.
+       
        intro HH.
        simpl in HH.
        destruct HH as [HH | HH].
-       simpl. left. easy.
-       simpl. right.
+       destruct HH as [HH | HH].
+       destruct HH as( H1a, H1b).
+       simpl. left. left. split; easy.
+       simpl. left. right. easy.
+       right.
        apply Ha1. easy.
-       
+
        intros.
        destruct Ha as (Ha1,Ha2).
        split. intro HH.
@@ -650,9 +743,24 @@ Proof. intros.
        destruct IHtyp_proc as (T',(G',(Ha,Hb))).
        exists T'. exists G'.
        split.
-       easy. 
+       
+       unfold eq_ctx in *.
+       split.
+       intros. split. intro Hc.
+       simpl.
+       destruct Ha as (Ha1, Ha2).
+       apply Ha1.
+       
+       admit.
+       admit.
+       intros.
+       split. intro Hc.
+       simpl.
+       admit.
+       admit.
+(*        easy.  *)
        specialize(stTrans T' t t' Hb H1); intro HT. easy.
-Qed.
+Admitted.
 
 Lemma _a23_f: forall P m em T G,
   typ_proc m em G P T ->
@@ -666,8 +774,11 @@ Proof. intros.
        apply st_mon.
 Qed.
 
-
-
+Lemma _a21: forall P Q m em T G,
+  typ_proc m em G Q T ->
+  typ_proc (S m) em (extendT G m T) P T ->
+  typ_proc m em G (subst_proc Q P) T.
+Proof. Admitted.
 
 
 
